# ๊ณฑ์๊ณต์์ ๋ณํ

### ์๋ฆฌ โ [์๊ณฑ์ ํฉ]

<aside>
๐ก (x + y)^2 = x^2 + 2xy + y^2
(x - y)^2 = x^2 - 2xy + y^2

x^2 + y^2 = (x + y)^2 - 2xy
x^2 + y^2 = (x - y)^2 + 2xy

</aside>

### ์์

1. ์ด๋ค ๋ ์ x, y์ ํฉ์ด 5์ด๊ณ ๊ณฑ์ด 10์ผ ๋, x^2 + y^2๋?

    x + y =5

    xy = 10,

    x^2 + y^2

    = (x + y)^2 - 2xy

    = 5^2 - 2 * 10

    = 25 - 10

    = 15


### ์๋ฆฌ โก [ํฉ์ ์๊ณฑ, ์ฐจ์ ์๊ณฑ]

<aside>
๐ก (x + y)^2 = x^2 + 2xy + y^2
x^2 + y^2 = (x + y)^2 - 2xy

(x - y)^2 = x^2 - 2xy + y^2
x^2 + y^2 = (x - y)^2 + 2xy

โด (x + y)^2 - 2xy = (x - y)^2 + 2xy

(x + y)^2 = (x - y)^2 + 4xy
(x - y)^2 = (x + y)^2 - 4xy

</aside>

### ์์

x + y =4, x^2 + y^2 = 10์ผ ๋, ๋ค์์?

1. xy

    (x + y)^2

    = x^2 + 2xy + y^2

     -2xy = 10

    xy = -5

2. (x - y)^2

    (x + y)^2 = (x - y)^2 + 4xy

    16 =  (x - y)^2 -20
